## 1998 April 03

**Instructions.** Do at least four problems in Part A, and at least two problems in Part B.

### PART A

1.  Let $\{xâ‚™\}_{n=1}^âˆ$ be a bounded sequence of real numbers, and for each positive
    $n$ define $\hat{x}_n = \sup_{k â‰¥ n} x_k$.

    a. Explain why the limit $â„“ = \lim_n \hat{x}_n$ exists.  
    b. Prove that for every $Ïµ > 0$ and every positive integer $N$ there exists an
       integer $k$ such that $k â‰¥ N$ and $| xâ‚– - â„“ | < Ïµ$.

2.  Let $C$ be a collection of subsets of the real line â„ and define
    
    $A_Ïƒ(C) = â‹‚ \{A : C âŠ† A \text{ and } A \text{ is a Ïƒ-algebra of subsets of } â„\}$.

    a.  Prove that $A_Ïƒ (C)$ is a Ïƒ-algebra, that $C âŠ† A_Ïƒ(C)$, and that $A_Ïƒ(C) âŠ† ğ”„$
        for every Ïƒ-algebra ğ”„ containing all the sets in $C$.  
    b.  Let $O$ be the collection of all finite open intervals in â„ and $F$ the
        collection of all finite closed intervals in â„.  Show that $A_Ïƒ(O) = A_Ïƒ(F)$.

3.  Let $(X, A, Î¼)$ be a measure space, and suppose $X = â‹ƒ_n X_n$, where
    $\{X_n\}_{n=1}^âˆ$ is a pairwise disjoint collection of measurable subsets of $X$.
    Use the Monotone Convergence Theorem and linearity of the integral to prove that,
    if $f$ is a nonnegative measurable real-valued function on $X$, then 
    $âˆ«_X f \, dÎ¼ = âˆ‘_n âˆ«_{X_n} f\, dÎ¼$.

4.  Using the Fubini/Tonelli Theorems to justify all steps, evaluate the integral
    $âˆ«_0^1 âˆ«_y^1 x^{-3/2} \cos \left(\frac{Ï€ y}{2x}\right) \, dx\, dy$.
   
5.  Let $I$ be the interval $[0, 1]$.  Let $C(I)$, $C(I Ã— I)$ denote the spaces of
    real valued continuous functions on $I$ and $I Ã— I$, respectively, with the
    usual supremum norm on these spaces.  Show that the collection of **finite** sums
    of the form $f(x, y) = âˆ‘_i Ï•_i(x) Ïˆ_i(y)$ (where $Ï•_i, Ïˆ_i âˆˆ C(I)$ for each $i$)
    is dense in $C(I Ã— I)$. 

6.  Let $m$ be Lebesgue measure on the real line â„, and for each Lebesgue
    measurable subset $E$ of â„ define $Î¼(E) = âˆ«_E \frac{1}{1+x^2}\, dm(x)$. 
    Show that $m$ is absolutely continuous with respect to $Î¼$, and
    compute the Radon-Nikodym derivative $dm/dÎ¼$. 

### PART B

7.  Let $Ï•(x,y) = x^2 y$ be defined on the square $S = [0, 1] Ã— [0, 1]$ in the plane,
    and let $m$ be two-dimensional Lebesgue measure on $S$.  Given a Borel subset $E$
    of the real line â„, define $Î¼(E) = m(Ï•^{-1}(E))$.

    a.  Show that $Î¼$ is a Borel measure on â„.  
    b.  Let $Ï‡_E$ denote the characteristic function of the set $E$.  Show that 
        $âˆ«_â„ Ï‡_E \, dÎ¼ = âˆ«_S Ï‡_E âˆ˜ Ï• \, dm$.  
    c.  Evaluate the integral $âˆ«_{-âˆ}^âˆ t^2 \, dÎ¼(t)$.
  
8.  Let $f$ be a real valued and increasing function on the real line â„, such that 
    $f(-âˆ) = 0$ and $f(âˆ) = 1$.  Prove that $f$ is absolutely continuous on every 
    closed finite interval if and only if $âˆ«_â„ f'\, dm = 1$.

9.  Let $F$ be a continuous linear functional on the space $L^1[-1, 1]$, with the 
    property that $F(f) = 0$ for all *odd* functions $f$ in $L^1[-1, 1]$.
    Show that there exists an *even* function $Ï•$ such that 
    $F(f) = âˆ«_{-1}^1 f(x) Ï•(x)\, dx$, for *all* $f âˆˆ L^1[-1, 1]$.  
    (*Hint*. One possible approach is to use the fact that any function in 
    $L^p[-1, 1]$ is the sum of an odd function and an even function.)

  

??? info "Solution A.3."

    Note that the hypotheses imply $Î½(E) = âˆ«_E f \, dÎ¼$ is a measure, 
    <!-- (problem 4, Nov.~'91), -->
    from which the desired conclusion immediately follows.  

    Of course, this does not answer the question as stated, since the examiners specifically 
    require the use of the MCT and linearity of the integral.

    Define $fâ‚™ = âˆ‘_{k=1}^n f Ï‡_{X_k} = f Ï‡_{âˆª_1^n X_k}$.
    
    Then it's clear that the hypotheses of the MCT are satisfied.  That is,
    $âˆ€ x âˆˆ X$,
    
    1. $0 â‰¤ fâ‚(x) â‰¤ fâ‚‚(x) â‰¤ â‹¯ â‰¤ f(x)$, and

    2. $\lim_n fâ‚™(x) = f(x) Ï‡_X(x) = f(x)$.

    Therefore, by linearity of the integral,

    $âˆ‘_{k=1}^âˆ âˆ«_{Xâ‚–} f\, dÎ¼ = \lim_n âˆ‘_{k=1}^n âˆ«_X f Ï‡_{Xâ‚–}\, dÎ¼\\
        = \lim_n âˆ«_X âˆ‘_{k=1}^n f Ï‡_{Xâ‚–}\, dÎ¼.$ 

    which, by definition of $fâ‚™$, is equal to $\lim_n âˆ«_X fâ‚™ \, dÎ¼$.
    
    By the MCT, $âˆ«_X \lim_n fâ‚™ \, dÎ¼ = âˆ«_X f\, dÎ¼$.
    
    âˆ

??? info "Solution A.4."

      By Tonelli's Theorem, if 
      1. $f(x,y) â‰¥ 0$ is measurable and
      2. one of the iterated integrals $âˆ¬ f(x,y)\,dx\,dy$ or $âˆ¬ f(x,y)\,dy\,dx$ exists,
      then they both exist and are equal.
      
      Moreover, if one of the iterated integrals is finite, then $f(x,y) âˆˆ L^1(dx,dy)$.

      Let $g(x, y) = x^{-3/2}\cos(\pi y/2x)$, and apply Tonelli's theorem to
      the non-negative measurable function $|g(x, y)|$ as follows:

      $âˆ«_0^1 âˆ«_0^x |g(x, y)| \, dy \, dx = âˆ«_0^1 âˆ«_0^x |x|^{-3/2} 
                                           \left|\cos\left(\frac{Ï€ y}{2x}\right)\right|\,dy\,dx
      â‰¤ âˆ«_0^1 âˆ«_0^x  x^{-3/2}\cdot 1 \,dy\,dx = âˆ«_0^1 x^{-1/2} \,dx = 2$.

      Thus one of the iterated integrals is finite, so $g(x, y) âˆˆ L^1(dx, dy)$ by Tonelli's theorem.
      
      Therefore, Fubini's Theorem applies to $g(x, y)$, and yields

      $âˆ«_0^1 âˆ«_y^1 x^{-3/2} \cos \left(\frac{Ï€ y}{2x}\right) \, dx \, dy 
      = âˆ«_0^1 âˆ«_0^x x^{-3/2}\cos\left(\frac{\pi y}{2x}\right)\,dy\,dx$.

      The latter is clearly equal to the first (hence the last) of the equivalent expressions below.

      $âˆ«_0^1 x^{-3/2} \cdot \frac{2x}{\pi} \left[\sin\left(\frac{\pi y}{2x}\right)\right]_{y=0}^{y=x} \, dx 
      = âˆ«_0^1 \frac{2}{\pi}x^{-1/2}\, dx = \frac{2}{Ï€} \left[2 x^{1/2}\right]_{x=0}^{x=1} = \frac{4}{Ï€}$.
      
      âˆ


??? info "Solution A.6"

      Obviously both measures are non-negative.  We must first prove $m â‰ª Î¼$.
      To this end, suppose $m(E) > 0$, where $E âˆˆ Ïƒ(m)$, the Ïƒ-algebra of Lebesgue measurable sets. 
      If we can show $Î¼(E) > 0$, this will establish that the implication 
      $Î¼(E) = 0 \, â‡’ \, m(E) = 0$ holds for all $E âˆˆ Ïƒ(m)$; i.e., $m â‰ª Î¼$.

      For $n = 1, 2, â€¦$, define $A_n = \{x âˆˆ â„ : \frac{1}{n+1} < \frac{1}{1+x^2} â‰¤ \frac{1}{n}\}$.

      Then $A_i âˆ© A_j = âˆ…$ for all $i â‰  j$ in â„•, and, for all $n = 1, 2, â€¦$,
      $Î¼(A_n) â‰¥ \frac{1}{n+1} m(A_n)$.

      Also, $â„ = â‹ƒ_n A_n$, since $0 < \frac{1}{1+x^2} \leq 1$ holds for all $x âˆˆ â„$.

      Therefore, $Î¼(E) = Î¼(E âˆ© â‹ƒ_n A_n) = Î¼(â‹ƒ_n (A_n âˆ© E)) = âˆ‘_n Î¼(A_n âˆ© E)$.

      The last equality might need a bit of justification. Since $f(x) = \frac{1}{1+x^2}$
      is continuous, hence measurable, the sets $\{A_n\}$ are measurable.  Therefore, the
      last equality holds by countable additivity of disjoint measurable sets.

      Note that $m(E) = âˆ‘_n m(A_n âˆ© E) > 0$ implies the existence of an $n âˆˆ â„•$
      such that $m(A_n âˆ© E) > 0$.  Therefore, 
      
      $Î¼(E) â‰¥ Î¼(A_n âˆ© E) â‰¥ \frac{1}{n+1} m(A_n âˆ© E) > 0$,

      which proves that $m â‰ª Î¼$.

      By the Radon-Nikodym Theorem there is a unique $h âˆˆ L^1(Î¼)$ such that
      
      $m(E) = âˆ« h \, dÎ¼$, and $âˆ« f\, dm  = âˆ« f \, h \, dÎ¼$, for all $f âˆˆ L^1(m)$.

      In particular, if $E âˆˆ Ïƒ(m)$ and $f(x) = \frac{1}{1+x^2} Ï‡_E$, then
      
      $Î¼(E) = âˆ«_E \frac{1}{1+x^2} \, dm(x) = âˆ«_E \frac{h(x)}{1+x^2}\, dÎ¼(x)$.

      That is, $âˆ«_E \, dÎ¼ = âˆ«_E \frac{h(x)}{1+x^2}\, dÎ¼(x)$ holds for all
      measurable sets $E$, which implies (see note blow) that, $\frac{h(x)}{1+x^2} = 1$ 
      holds for $Î¼$-almost every $x âˆˆ â„$.  Therefore, $\frac{dm}{dÎ¼}(x) = h(x) = 1+x^2$.
      
      âˆ

      **Remarks**.  

      +  The penultimate implication comes from the following standard result: if $f$ and
         $g$ are integrable functions such that $âˆ«_E f = âˆ«_E g$ holds for all measurable
         sets $E$, then $f = g$, $Î¼$-a.e.  

      +  $h$ is uniquely defined only up to an equivalence class of functions
         that are equal to $1+x^2$, $Î¼$-a.e. 

??? info "Solution B.2."

      **Preliminary remark**.  I have worked this problem a number of times, and what 
      follows is the clearest and most instructive proof I have come up with.  It is 
      by no means the shortest, most elegant solution, and probably not the type of
      detailed answer one ought to provide on an actual exam, when time is a factor.
      However, some of the facts that I prove in detail here have appeared as separate
      questions on other exams, so the proofs are worth knowing.

      Note that $f$ is increasing, so $f'$ exists for a.e. $x âˆˆ â„$
      and $f'(x) â‰¥ 0$ wherever $f'$ exists.  Also, $f'$ is measurable.  To
      see this, define
      
      $g(x) = \limsup_{n â†’ âˆ} \, [f(x+ \frac{1}{n})-f(x)] \, n$.

      As a lim sup of a sequence of measurable functions, $g$ is measurable
      (Theorem 1.14 of Rudin (1987)).

      Let $E$ be the set on which $f'$ exists.  Then
      $m(â„ - E) = 0$, and $f' = g$ on $E$ (by definition of derivative),
      so $f'$ is measurable.

      +  (â‡) Suppose $âˆ«_â„ f' \, dm = 1$.  We must show $f âˆˆ AC[a, b]$
         for all $-âˆ < a < b < âˆ$.  First, check that $f' âˆˆ L^1(â„)$, since

         $1 = âˆ«_â„ f' \, dm  = âˆ«_{â„ - E} f' \, dm + âˆ«_E f' \, dm = âˆ«_E f' \, dm$,

         (The last equality holds because $m(â„ - E) = 0$.)

         Since $f$ is increasing, $f' â‰¥ 0$ on $E$, so

         $âˆ«_â„ |f'| \, dm  = âˆ«_{â„ - E} |f'| \, dm + âˆ«_E |f'| \, dm = âˆ«_E |f'| \, dm =  âˆ«_E f' dm = 1$.

         Thus, $f' âˆˆ L^1(â„)$ as claimed.

         A couple of lemmas will be needed to complete the â‡ direction of the proof.
         The first is proved in the appendix
         <!-- (sec.~\ref{sec:miscellaneous-proofs}),  -->
         while the second can be found on page 100 of Royden (1988). 
         <!-- , ~\cite{Royden:1988} on page~100. -->

         **Lemma 8.1**.  <!-- \label{lemma:8-1}   -->
         Let $f: â„ â†’ â„$ be a function.  If $f$ is differentiable on $[a, b]$, 
         $f' âˆˆ L^1([a, b])$, and $âˆ«_a^x f'(t) \, dt = f(x) - f(a)$ for $a â‰¤ x â‰¤ b$, 
         then $f âˆˆ AC[a,b]$.

         The converse of this lemma is also true. 

         See Folland (1999) for a nice treatment of the Fundamental Theorem of Calculus (FTC) for Lebesgue integration. 
         
         **Lemma 8.2**. If $f: â„ â†’ â„$ is increasing and $f' âˆˆ L^1([a,b])$, then
         $âˆ«_a^x f'(t) \, dt â‰¤ f(x) - f(a)$.

         To finish the â‡ direction of the proof, by Lemma 8.1, it suffices to show that 
         $âˆ«_â„ f' \, dm = 1$ implies $âˆ«_a^b f'(t) \, dt = f(b) - f(a)$ holds for all 
         $-âˆ < a < b < âˆ$.
         
         By Lemma 8.2, we have $âˆ«_a^b f'(t) \, dt â‰¤ f(b) - f(a)$, so we need
         only show that strict inequality cannot hold.
         
         Suppose, by way of contradiction, that $âˆ«_a^b f'(t) \, dt < f(b) - f(a)$ 
         holds for some $-âˆ < a < b < âˆ$.  Then,

         $1 = âˆ«_â„ f' \, dm = âˆ«_{-âˆ}^a f' \, dm + âˆ«_a^b f' \, dm + âˆ«_b^âˆ f' \, dm$

         $< [f(a) - f(-âˆ)] + [f(b) - f(a)] + [f(âˆ) - f(b)] = f(âˆ) - f(-âˆ) = 1$.

         Therefore, $âˆ«_â„ f' \, dm = 1$ implies that

         $âˆ«_a^b f'(t) \, dt = f(b) - f(a)$ holds for all $-âˆ < a < b < âˆ$, as desired.

      +  (â‡’) Assume $f âˆˆ AC[a, b]$ for all $-âˆ < a < b < âˆ$. We must show 
         $âˆ«_â„ f' \, dm = 1$.  By assumption $f(âˆ) - f(-âˆ) = 1$, so this
         is equivalent to showing
      
         $\lim_{x â†’ âˆ} âˆ«_{-x}^x f'(t) dm(t) = \lim_{x â†’ âˆ}[f(x) - f(-x)]$.
      
         Let $xâˆˆ â„$, $x > 0$, and $f âˆˆ AC[-x,x]$.  We claim
         $f(x)-f(-x) = âˆ«_{-x}^x f' dm$.  Assuming the claim is true---see
         p. 110 of Royden (1988) for the proof---we have

         $1 = \lim_{x â†’ âˆ} [f(x) - f(-x)] = \lim_{x â†’ âˆ}âˆ«_{-x}^x f'(t) dm(t) = âˆ«_â„ f' dm$.
         
         âˆ

??? info "Solution B.3."

      Since $F âˆˆ L^1[-1, 1]^*$, then by the Riesz Representation Theorem
      <!-- \footnote{See problem~\ref{item:2001-3-1} of section~\ref{sec:2001-november-26}.} -->
      there is a unique $h âˆˆ L^âˆ[-1,1]$ such that
      
      $F(f) = âˆ«^1_{-1} f(x) h(x) \, dx$ for all $f âˆˆ L^1[-1,1]$.

      Let $h = Ï• + Ïˆ$, where $Ï•$ and $Ïˆ$ are the even and odd functions,
      
      $Ï•(x) = \frac{h(x) + h(-x)}{2}$ and $Ïˆ(x) = \frac{h(x) - h(-x)}{2}$.
      
      Let $f = f_e + f_o$ be the decomposition of $f$ into a sum of even and odd
      functions.  Then, by linearity of $F$, and since $F(f_o) = 0$ by hypothesis,
      
      $F(f) = F(f_e) + F(f_o) = F(f_e) = âˆ«_{-1}^1 f_e h = âˆ«_{-1}^1 f_e Ï• +âˆ«_{-1}^1 f_e Ïˆ$.
      
      Now note that $f_e Ïˆ$ is an odd function (even times odd), so $âˆ«_{-1}^1 f_e Ïˆ = 0$, 
      since $[-1, 1]$ is symmetric.  Similarly, $âˆ«_{-1}^1 f_o Ï• = 0$. Therefore,
      
      $F(f) = F(f_e) = âˆ«_{-1}^1 f_e Ï• = âˆ«_{-1}^1 f_e Ï• + âˆ«_{-1}^1 f_o Ï• = âˆ«_{-1}^1 (f_e+f_o) Ï• = âˆ«_{-1}^1 f Ï•$.

      âˆ

