+++
title = "Real Analysis Exam"
description = "A part of the phd exam in analysis"
date = 2007-11-16
+++

## 2007 November 16

<!-- This was the exam I passed.  I was asked to re-write solutions to problems 1, 2, 4, and a modified (harder/more general) version of problem 6. -->

**Notation.** $\mathbb R$ is the set of real numbers and $\mathbb R^n$ is $n$-dimensional Euclidean space.  Denote by $m$ Lebesgue measure on $\mathbb R$ and $m_n$ $n$-dimensional Lebesgue measure. Be sure to give a *complete statement* of any theorems from analysis that you use in your proofs below. 

1. Let $\mu$ be a positive measure on a measure space $X$.  Assume that $E_1, E_2, \dots$ are measurable subsets of $X$ with the property that for $n\neq m, \mu(E_n\cap E_m) = 0$.  Let $E$ be the union of these sets.  Prove that $\mu(E) = \sum\_{n=1}^\infty \mu(E\_n)$.


2. (a) State a theorem that illustrates Littlewood's Principle for pointwise a.e. convergence of a sequence of functions on $\mathbb R$.\
   (b) Suppose that $f_n \in L^1(m)$ for $n=1,2,\dots$. Assuming that $\\|f\_n-f\\|\_1 \to 0$ and $f_n \to g$ a.e. as $n\to \infty$, what relation exists between $f$ and $g$?  Make a conjecture and then prove it using the statement in Part (a).
<!-- \index{Egoroff's theorem!problems|(}   -->

3. Let $K$ be a compact subset in $\mathbb R^3$ and let $f(x) = \mbox{dist}(x,K)$.\
   (a) Prove that $f$ is a continuous function and that $f(x) = 0$ if and only if $x\in K$.\
   (b) Let $g = \max \\{1-f, 0\\}$ and prove that $\lim\_{n\to \infty} \iiint g^n$ exists and is equal to $m_3(K)$.

4. Let $E$ be a Borel subset of $\mathbb R^2$.\
   (a) Explain what this means.\
   (b) Suppose that for every real number $t$ the set $E_t = \\{(x,y) \in E \mid x=t\\}$ is finite.  Prove that $E$ is a Lebesgue null set.

5. Let $\mu$ and $\nu$ be finite positive measures on the measurable space $(X,\mathcal A)$ such that $\nu \ll \mu \ll \nu$, and let $d\nu/d(\mu + \nu)$ denote the Radon-Nikodym derivative of $\nu$ with respect to $\mu+\nu$.  Show that 
$$0 < \frac{d\nu}{d(\mu + \nu)} < 1 \quad \text{a.e.} [\mu].$$
  <!-- \index{Radon-Nikodym!problems} -->

6. Suppose that $1 < p < \infty$ and $q = p/(p-1)$ and let $a_1, a_2, \dots$ be a sequence of real numbers for which the series $\sum a_n b_n$ converges for all real sequences $\{b_n\}$ satisfying the condition $\sum |b_n|^q < \infty$.\
   (a) Prove that $\sum |a_n|^p < \infty$.\
   (b) Discuss the cases of $p=1$ and $p=\infty$.  Prove your assertions.
<!-- On the original exam this question asked only about the special case $p=q=2$. -->
   

<!-- 
SOLUTION 1.
  \ifthenelse{\boolean{includeSolutions}}{\begin{solution}
      Define $F_1 = E_1, \, F_2 = E_2 \setminus E_1,\, F_3 = E_3 \setminus (E_1 \cup
      E_2), \dots $, and, in general, 
      \[
      F_n = E_n \setminus \bigcup_{i=1}^{n-1} E_i \quad (n=2, 3, \dots).
      \]
      If $\sigM$ is the \sigalg\ of $\mu$-measurable subsets of $X,$ then
      $F_n\in \sigM$ for each $n\in \N,$ since $\sigM$ is a \sigalg.  
      Also, $F_i\cap F_j = \emptyset$ for $i\neq j$, and 
      $F_1\cup F_2 \cup \cdots \cup F_n = E_1\cup E_2 \cup \cdots \cup E_n$ 
      for all $n\in \N$. Thus,
      \[
      \bigcup_{n=1}^\infty F_n = \bigcup_{n=1}^\infty E_n \triangleq E,
      \]
      and, by $\sigma$-additivity of $\mu$, 
      \[
      \mu(E) = \mu(\bigcup_{n=1}^\infty F_n) = \sum_{n=1}^\infty \mu(F_n).
      \]
      Therefore, if we can show $\mu(E_n) = \mu(F_n)$ holds for all $n\in \N$,
      the proof will be complete.  

      Now,  for each $n = 2, 3, \dots$,
      \begin{equation}
        \label{eq:2007-11-1a}
        F_n = E_n \cap (\bigcup_{i=1}^{n-1}E_i)^c
      \end{equation}
      and
      \begin{equation}
        \label{eq:2007-11-1b}
        \mu(E_n) = \mu(E_n \cap (\bigcup_{i=1}^{n-1}E_i)^c) + \mu(E_n \cap
        (\bigcup_{i=1}^{n-1}E_i)).
      \end{equation}
      Equation (\ref{eq:2007-11-1b}) holds because
      $\bigcup_{i=1}^{n-1}E_i$ is a measurable set for each $n = 2, 3, \dots$. 
      Finally, note that
      \[
      E_n \cap (\bigcup_{i=1}^{n-1}E_i) =    \bigcup_{i=1}^{n-1}(E_n\cap E_i),
      \]
      which implies 
      \[
      \mu(E_n \cap (\bigcup_{i=1}^{n-1}E_i)) \leq \sum_{i=1}^{n-1}\mu(E_n\cap E_i),
      \]
      by $\sigma$-subadditivity.  By assumption, each term in the last sum is zero, and
      therefore, by (\ref{eq:2007-11-1a}) and~(\ref{eq:2007-11-1b}),
      \[
      \mu(E_n) = \mu(E_n \cap (\bigcup_{i=1}^{n-1}E_i)^c)  = \mu(F_n) \quad \text{holds
        for each $n=2, 3, \dots$}.
      \]
      For $n=1$, we have $F_1 = E_1$, by definition.  This completes the proof.
      \qed
    \end{solution}  }{}

  \pspace 



SOLUTION 2.

\ifthenelse{\boolean{includeSolutions}}{\begin{solution}~\\
      {\bf (a)} I think it's generally accepted that the Littlewood principle dealing with
      a.e.~convergence of a sequence of functions on $\mathbb R$ is Egoroff's theorem, which is
      stated below in section \ref{thm:egoroff}.\\[6pt]
      {\bf (b)} {\it Conjecture:} $f = g$ a.e.\\[6pt]
      {\it Proof 1}:\footnote{Note that {\it Proof 1}, which
        seems to me the more natural one, doesn't use Egoroff's theorem, so
        either the examiners were looking for a different proof, or a different
        conjecture, or perhaps Egoroff's theorem was not the Littlewood principle they
        had in mind.  In any event, I have found a way to prove the conjecture
        which does make use of Egoroff's theorem, and this appears here as {\it Proof 2}.}
      First recall %the easily proved, yet important theorem which states 
      that $L^1$ convergence implies convergence in measure. That is, if 
      $\{f_n\} \subset L^1(m)$ and $\|f_n-f\|_1 \to 0$, then $f_n 
      \to f$ in measure. (Proof: 
      $m(\{x:|f_n(x) - f(x)| >\epsilon\}) \leq \frac{1}{\epsilon}\|f_n-f\|_1 \to
      0.$) Next recall another important theorem\footnote{Folland~\cite{Folland:1999},
        theorem 2.30 and its corollary.} which states that if $f_n\to f$ in measure
      then there is a subsequence $\{f_{n_j}\} \subseteq \{f_n\}$ which converges a.e.~to $f$
      as $j\to \infty$.  Combining these two results in the
      present context (Lebesgue measure on the real line), we can say the
      following:\footnote{Perhaps this statement is the version of the Littlewood principle
        dealing with a.e.~convergence that we were meant to cite in part (a).}
      If $\{f_n\} \subset L^1(m)$ and $\|f_n-f\|_1\to 0$ then there is a
      subsequence $\{f_{n_j}\} \subseteq \{f_n\}$ with the property $f_{n_j}(x)
      \to f(x)$ for almost all $x\in \mathbb R$.

      Now, if $f_n(x)\to g(x)$ for almost all $x\in \mathbb R$, and if $B_1$ be the set
      of measure zero where $f_n(x) \nrightarrow g(x)$, then off of $B_1$ the sequence
      $f_n$, as well as every subsequence of $f_n$, converges to $g$. 
      Let $\{f_{n_j}\}$ be the subsequence mentioned above which converges to $f$ almost
      everywhere.  Then  
      \begin{equation}
        \label{eq:2007-2-1}
        |f(x) - g(x)| \leq 
        |f(x) - f_{n_j}(x)|+
        |f_{n_j}(x) - g(x)|.
      \end{equation}
      Define $B_2 = \{x\in \mathbb R:f_{n_j}(x) \nrightarrow f(x)\}$.  Then the set $B = B_1 \cup
      B_2$ has measure zero and, for all $x\in $\mathbb R$setminus B$, 
      $f_{n_j}(x)\to f(x)$ and $f_{n_j}(x)\to g(x)$ .  
      Therefore, by (\ref{eq:2007-2-1}), $|f(x) -g(x)| = 0$ for
      all $x\in $\mathbb R$setminus B$. It follows that the set
      $\{x\in \mathbb R:f_(x) \neq g(x)\} \subset B$, as a subset of a null set, must itself be a
      null set (since $m$ is complete). 
      That is, $f = g$ a.e.~and the conjecture is proved.
      \qed~\\[2pt]
      {\it Proof 2:}
      First, we claim that if $f = g$ a.e.~on $[-n,n]$ for every $n\in \N$, then
      $f=g$ a.e.~in \mathbb R.  To see this, let $B_n = \{x\in [-n,n]: f(x) \neq g(x)\}$.  Then
      $mB_n = 0$ for all $n\in \N$, so that if $B = \{x\in \mathbb R:f(x) \neq g(x)\}$, then $B =
      \cup B_n$ and $mB \leq \sum m B_n = 0$, as claimed.
      Thus, to prove the conjecture, it is enough to show that $f = g$ for almost every
      $-n \leq x \leq n$, for an arbitrary fixed $n\in \N$.

      Fix $n\in \N$, and suppose we know that $f - g \in L^1([-n,n], m)$. 
      (This will follow from the fact that $f, g \in L^1([-n,n],m)$, 
      which we prove below.)  Then, for all $\epsilon >0$ there is a
      $\delta >0$ such that $\int_E |f-g|\, dm < \epsilon$ for all measurable $E\subseteq
      [-n,n]$ with $mE < \delta$.  Now apply Egoroff's theorem to find a set $A \subseteq [-n,n]$
      such that $m([-n,n]\setminus A)< \delta$ and $f_n\to g$ uniformly on $A$. Then 
      \begin{align*}
        \int_{-n}^n |f-g|\, dm &= 
        \int_{[-n,n]\setminus A} |f-g|\, dm + \int_{A} |f-g|\, dm \\
        &\leq \epsilon + \int_{A} |f-f_n|\, dm + \int_{A} |f_n-g|\, dm \\
        &\leq \epsilon + \|f-f_n\|_1 + mA\, \sup_{x\in A}|f_n(x)-g(x)|,
      \end{align*}  
      where $\|f-f_n\|_1\to 0$, by assumption, and 
      $\sup_{x\in A}|f_n(x)-g(x)| \to 0$ 
      since $f_n\to g$ uniformly on $A$. 
      Since $\epsilon >0$ was arbitrary, it
      follows that $\int_{-n}^n |f - g| \, dm = 0$ and, for functions
      $f, g \in L^1([-n,n],m)$, this implies that $f = g$ a.e.~on $[-n,n]$.

      It remains to show that $f, g \in L^1([-n,n],m)$.  It's clear that $f\in L^1$ since
      $\|f\|_1 \leq \|f - f_n\|_1 + \|f_n\|_1 < \infty$.  To prove $g \in L^1([-n,n],m)$
      note that $f_n \xrightarrow{a.e.} g$ implies 
      $\lim_n |f_n(x)| =|g(x)|$ for almost all $x$, so by Fatou's lemma,
      \[
      \|g\|_1 = \int |g|\, dm = \int \varliminf |f_n| \, dm \leq \varliminf \int |f_n| \,
      dm = \lim \|f_n\|_1 = \|f\|_1 < \infty.
      \]
      The last equality holds because, by the triangle inequality,
      $\left| \|f_n\|_1 - \|f\|_1 \right| \leq \|f_n - f\|_1 \to 0$.
      \qed
      \index{Egoroff's theorem!problems|)}
    \end{solution}  }{}

  \pspace 

SOLUTION 3.
  \ifthenelse{\boolean{includeSolutions}}{\begin{solution}
      {\bf (a)} Define $\mbox{dist}(x,K) = f(x) = \inf_{k\in K} |x-k|$.
      Clearly, for all $k\in K$, 
      % $d(x,K) \leq |x-k|$.  Therefore, 
      $f(x) \leq |x-k|$.  Therefore, 
      by the triangle inequality, for any $x, y\in \mathbb R^3$, 
      \[
      % d(x,K) \leq |x-y|+|y-k|, \quad \forall k\in K,
      f(x) \leq |x-y|+|y-k|, \quad \forall k\in K,
      \]
      and so, taking the infimum over $k\in K$ on the right,
      \begin{equation}
        \label{eq:2007-3-1}
        % d(x,K) \leq |x-y|+d(y,K).  
        f(x) \leq |x-y|+f(y).  
      \end{equation}
      Similarly,
      \begin{equation}
        \label{eq:2007-3-2}
        % d(y,K) \leq |x-y|+d(x,K).
        f(y) \leq |x-y|+f(x).
      \end{equation}
      Obviously, for any given $x\in \mathbb R^3$,
      % $d(x,K)$ 
      $f(x)$ is finite. 
      Therefore, (\ref{eq:2007-3-1}) and (\ref{eq:2007-3-2}) together imply that
      \[
      % |d(x,K)-d(y,K)| \leq |x-y|.
      |f(x)-f(y)| \leq |x-y|, \quad \forall\, x, y \in \mathbb R^3.
      \]
      Whence $f$ is (Lipschitz) continuous. 

      Now, if $x\in K$, then it's clear that $f(x) = 0$. Suppose $x \notin K$; that is, $x$
      is in the complement $K^c$ of $K$.  Since $K$ is closed, $K^c$ is open and we can find an
      $\epsilon$-neighborhood about $x$ fully contained in $K^c$, in which case 
      $f(x) > \epsilon$.  We have thus proved that $f(x) = 0$ if and only if $x\in K$.
      \qed~\\[4pt]
      \index{dominated convergence theorem!applied}
      {\bf (b)} First observe that $f(x)=0$ for all $x\in K$, and 
      $f(x)>0$ for all $x\notin K$.  Define $K_1$ to be a closed and bounded set containing
      $K$ on which $f(x) \leq 1$.  That is, $K_1$ is the set of points that are a
      distance of not more than 1 unit from the set $K$.  In particular $K \subset K_1$.
      Notice that $g = \max(1-f,0) = (1-f)\chi_{K_1}$. Also, if $x\in
      K_1\setminus K$, then $0\leq 1-f(x) < 1$, so $g^n\to 0$ on the set $K_1
      \setminus K$, while on the set $K$, $g^n = 1$ for all $n\in \N$.  Therefore, $g^n
      \to \chi_K$.  Finally, note that $g^n \leq \chi_{K_1}\in L^1(\mathbb R^3)$ so the
      dominated convergence theorem can be applied to yield
      $\lim_{n\to \infty} \iiint g^n
      = \iiint \chi_K = m_3(K).$
      \qed
    \end{solution}  }{}

%  \ifthenelse{\boolean{newpagebetweenexams}}{\newpage}{\btwnexamspace}
\pspace

SOLUTION 4.
  \ifthenelse{\boolean{includeSolutions}}{\begin{solution}~\\
      {\bf (a)} The \emph{Borel} $\sigma$\emph{-algebra} of $\mathbb R^2$, which we denote by
      \index{Borel $\sigma$-algebra}
      $\borel(\mathbb R^2)$, is the smallest $\sigma$-algebra that contains the
      open subsets of $\mathbb R^2$.  
      \index{Borel set}
      The sets belonging to $\borel(\mathbb R^2)$ are called \emph{Borel subsets} of
      $\mathbb R^2$.\\[4pt]
      {\bf (b)} First observe that if $G$ is a finite subset of $\mathbb R$, then $G$ is a Lebesgue
      null set.  That is, $mG = 0$.  In fact, it is easy to prove that if $G$ is any
      countable subset, then $mG = 0$. (Just fix $\epsilon >0$ and
      cover each point $x_n \in G$ with a set $E_n$ of measure less than 
      $\epsilon 2^{-n}$.  Then $mG \leq \sum mE_n < \epsilon$.)

      In problems involving 2-dimensional Lebesgue measure, distinguishing $x$ and $y$
      coordinates sometimes clarifies things. To wit, let
      $(X, \borel(X), \mu) = (Y, \borel(Y), \nu)$
      be two identical copies of the measure space 
      $(\mathbb R, \borel(\mathbb R), m)$, and represent Lebesgue measure on $\mathbb R^2$ by\footnote{The
        notation $\borel(X)\otimes \borel(Y)$ denotes the $\sigma$-algebra 
        generated by all sets $A \times B \subseteq X\times Y$ with $A \in \borel(X)$
        and $B\in \borel(Y)$. See~\ref{sec:fubini-tonelli}. 
        % \NTS{} 
        In this case, $\borel(X)\otimes \borel(Y)$ is the same as
        $\borel(\mathbb R^2)$.} 
      % (In general, the direct product of all sets from $\borel(X)$ with all sets from
      % $\borel(Y)$ does not form a $\sigma$-algebra.)  Of course, $\mu \times \nu$ denotes
      % the product measure on this $\sigma$-algebra.} 
      % 
      $(X\times Y, \borel(X)\otimes \borel(Y), \mu \times \nu) =(\mathbb R^2,\borel(\mathbb R^2), m_2)$.
      % $(X\times Y, \borel(\mathbb R^2), \mu \times \nu) = (\mathbb R^2, \borel(\mathbb R^2), m_2)$.

      Our goal is to prove that $m_2 E = 0$.  First note that 
      \[
      m_2 E = (\mu\times \nu)(E) = \int_{X\times Y} \chi_E \, d(\mu\times \nu).
      \]
      The integrand $\chi_E$ is non-negative and measurable (since $E$ is Borel).
      Therefore, by Tonelli's theorem~(\ref{thm:Fubini}),
      \begin{equation}
        \label{eq:200711-4-1}
        m_2 E = \int_Y \int_X \chi_E(x,y) \, d\mu(x)\, d\nu(y)
        = \int_X \int_Y \chi_E(x,y) \, d\nu(y) \, d\mu(x).
      \end{equation}
      Now, let 
      \[
      G_t = \{y\in \mathbb R: (x,y)\in E \text{ and } x=t\}.
      \]
      This is the so called ``$x$-section'' of $E$ at the point $x=t$.  It is a subset
      of $\mathbb R$, but we can view it as a subset of $\mathbb R^2$ by simply identifying each
      point $y\in G_t$ with the point $(t,y) \in E_t = \{(x,y)\in E: x = t\}$.
      It follows that, for each $t\in \mathbb R$, $G_t$ is a finite subset of $\mathbb R$.
      Therefore, $m G_t = 0$.  Finally, by~(\ref{eq:200711-4-1}),
      \[
      m_2 E = \int_X \int_Y \chi_{G_t}(y) \, d\nu(y) \, d\mu(t)
      = \int_X \nu G_t \, d\mu(t) = 0.
      \]
      since $\nu G_t \triangleq m G_t = 0$.
      \qed
    \end{solution}  }{}

  \pspace 

SOLUTION 5.
  \ifthenelse{\boolean{includeSolutions}}{\begin{solution}
      First note that $\nu \ll \mu$ implies $\nu \ll \mu+ \nu$, so, by the
      Radon-Nikodym theorem~(\ref{thm:radon-nikodym}), there is a unique 
      $f\in L^1(\mu+\nu)$ such that 
      \[
      \nu(E) = \int_E f \, d(\mu+\nu) \quad \forall E\in \sigA.
      \]
      Indeed, $f$ is the Radon-Nikodym derivative; \ie 
      $f = \frac{d\nu}{d(\mu + \nu)}$.  
      We want to show $0 < f(x) < 1$ holds for $\mu$-almost every $x\in X$.
      Since we're dealing with positive measures, we can assume $f(x)\geq 0$ for all
      $x\in X$.

      If $B_0 = \{x\in X: f(x) = 0\}$, then 
      \[
      \nu(B_0) = \int_{B_0} f \, d(\mu+\nu) = 0.
      \]
      Therefore, $\mu(B_0) = 0$, since $\mu \ll \nu$, which proves that $f(x) > 0$, $[\mu]$-a.e.  
      
      If $B_1 = \{x\in X: f(x) \geq 1\}$, then 
      \[
      \nu(B_1) = \int_{B_1} f \, d(\mu+\nu) \geq 
      (\mu+\nu)(B_1) = \mu(B_1)+\nu(B_1).
      \]
      Since $\nu$ is finite by assumption, we can subtract $\nu(B_0)$ from both sides
      to obtain $\mu(B_1) = 0$.  This proves $f(x) < 1$, $[\mu]$-a.e.  
      \qed
    \end{solution}  }{}

  \pspace

SOLUTION 6.
     \ifthenelse{\boolean{includeSolutions}}{\begin{solution}
      {\bf (a)} For each $k\in \N$, define $T_k : \ell_q(\N) \to \mathbb R$ by $T_k(b) = \sum_{n=1}^k a_n b_n$, 
      for $b\in \ell_q(\N)$.  Then  
      $\{T_k\}$ is a family of pointwise bounded linear functionals.  
      That is, each $T_k$ is a linear functional, and,
      for each $b\in \ell_q(\N)$, there is an $M_b \geq 0$ such
      that $|T_k(b)|\leq M_b$ holds for all $k\in \N$.  To see this, simply note that a
      convergent sequence of real numbers is bounded, and, in the present case, we have
      \[
      S_k \triangleq \sum_{n=1}^k a_n b_n \mathbb Rightarrow \sum_{n=1}^\infty a_n b_n =x \in
      \mathbb R. 
      \]
      Thus, $\{T_k(b)\} = \{S_k\}$ is a convergent sequence of reals, so, 
      if $N\in \N$ is such that $k\geq N$ implies $|S_k - x| < 1$, and if 
      $M_b'$ is defined to be $\max\{|S_k|: 1\leq k\leq N\}$, then, for any $k\in \N$,
      \[
      |T_k(b)| \leq M_b \triangleq \max\{ M_b', x+1\}.
      \]

      \index{Banach space!$\ell_p$}    
      % \index{Banach-Steinhauss|see{uniform boundedness principle}}
      \index{Banach-Steinhauss theorem}
      \index{uniform boundedness principle}

      Next note that $\ell_q$ is a Banach space, so the (Banach-Steinhauss) principle
      of uniform boundedness implies that there is a single $M>0$ such that 
      $\|T_k\| \leq M$ for all $k\in \N$.  In other words, 
      \[
      (\exists\, M>0) \, (\forall b\in \ell_q)\, (\forall k\in \N) \; |T_k(b)|\leq
      M\|b\|.
      \]
      Define let $T(b) \triangleq \sum_{n=1}^\infty a_n b_n = \lim_{k\to \infty}
      T_k(b)$, which exists by assumption.  Since $| \cdot |$ is continuous,
      we conclude that $\lim_{k\to \infty}|T_k(b)| =
      |T(b)|$. Finally, since $|T_k(b)| \leq M \|b\|$ for all $k\in \N$, we have 
      $|T(b)| \leq M \|b\|$.  That is $T$ is a bounded linear functional on
      $\ell_q(\N)$. 

      \index{Riesz representation theorem|(}
      Now, by the Riesz representation theorem, if $1\leq q < \infty$, then any bounded 
      linear functional $T\in \ell_q^*$ is uniquely representable by some
      $\alpha = (\alpha_1, \alpha_2, \dots) \in \ell_p$ as
      \begin{equation}
        \label{eq:RRT-20070601}
        T(b) = \sum_{n=1}^\infty \alpha_n b_n.
      \end{equation}    
      On the other hand, by definition, 
      $T(b) = \sum_{n=1}^\infty a_n b_n$, for all $b\in \ell_q$. Since the
      representation in (\ref{eq:RRT-20070601}) is unique, $a = \alpha \in \ell_p$.
      That is, $\sum_n |a_n|^p <\infty$. 
      \qed~\\[4pt]
      {\bf (b)} Consider the case $p=1$ and $q=\infty$.  First recall that the Riesz
      representation theorem says that every $T \in \ell_q^* \, (1\leq q < \infty)$ is
      uniquely representable by some $\alpha \in \ell_p$ (where $p = q/(q-1)$, 
      so $1<p\leq \infty$).  That is $\ell_p$ is the dual of $\ell_q$, when 
      $1\leq q<\infty$ and $p = q/(q-1)$.  However, in the present case we have
      $q=\infty$ and $p=1$ and $\ell_1$ is \emph{not} the dual of
      $\ell_\infty$. (Perhaps the easiest way to see this is to note that $\ell_1$ is
      separable but $\ell_\infty$ is not.  For the collection of $a\in \ell_\infty$
      such that $a_n\in \{0, 1\}, \,n\in \N$, is uncountable and, for any two distinct
      such sequences $a, b\in \{0, 1\}^{\N}$, we have $\|a - b\|_\infty = 1$, so there
      cannot be a countable base, so $\ell_\infty$ is not second countable, and a metric
      space is separable iff it is second countable.)

      So we can't use the same method of proof for this case.  However, I believe the
      result still holds by the following simple argument: Define $b = (b_1, b_2, \dots)$ by 
      \[
      b_n = \mbox{sgn}(a_n) =
      \begin{cases}
        \bar{a}_n/|a_n|, & \text{ for $a_n\neq 0$,}\\
        0, & \text{ for $a_n= 0$,}
      \end{cases}\quad (n\in \N).
      \]
      Then
      $\sum_n |a_n| = \sum_n a_n b_n$ converges by the hypothesis, since $|b_n| \in \{0, 1\}$ implies
      $b\in \ell_\infty$.  Therefore, $a\in \ell_1$.\\[4pt]

      Finally, in case $p=\infty$ and $q=1$, the Riesz representation theorem can be applied as
      in part (a).
      \qed
      \index{Riesz representation theorem|)}
    \end{solution}  }{}
\end{enumerate}

\pspace 
 -->
