+++
title="Ring Theory Exam"
date = 1992-11-01
+++

## 1992 November
1. a. Define ``injective module.''
   b. Prove: The module $Q$ is injective if every diagram with exact row

      (missing diagram)

      with **projective** $P$ is embeddable in a commutative diagram

      (missing diagram)



2. Let $R$ be a commutative ring with identity.  Recall that an ideal $P\subset R$ is said to be **prime** if $P\neq R$ and $ab \in P$ implies $a\in P$ or $b\in P$. Let $J\subseteq R$ be an ideal.
   a. Show that $J$ is prime if and only if $R/J$ is an integral domain.
   b. Show that $J$ is maximal if and only if $R/J$ is a field.
  
   (This is problem 2 of the April 2008 exam; see section (#sec:2008Apr).)

3. Let $R$ be a principal ideal domain.  Let $J_1 \subseteq J_2 \subseteq \cdots \subseteq J_i \subseteq J_{i+1}\subseteq \cdots$ be a chain of ideals in $R$. Show that there is an integer $n\geq 1$ such that $J_i = J_n$ for all $i\geq n$.


4. Let $R$ be a ring and $M$ a (left) $R$-module.  Suppose $M = K \oplus L$ and $\varphi$ is an $R$-endomorphism of $M$ with the property that $\varphi(L)\subseteq K$.  Prove that $M = K \oplus (1_M + \varphi)(L)$.

5. Let $R$ be any ring, $M, N, K$ submodules of some $R$-module such that $N\leq M$. Prove that the sequence 
   $$0 \longrightarrow \frac{M\cap K}{N\cap K} \longrightarrow \frac{M}{N} \longrightarrow \frac{M+ K}{N+ K} \longrightarrow 0$$
   is exact where the maps are the natural (obvious) ones.

6. Let $F$ be a field and let $R = F(X,Y]$ be the polynomial ring over $F$ in indeterminates $X, Y$.  Let $\alpha, \beta \in F$, and let $\varphi : R\rightarrow F$ be defined by $\varphi(f(X,Y)) = f(\alpha, \beta)$ for all polynomials $f(X,Y)\in R$.  Show that $\ker(\varphi) = (x-\alpha, y-\beta)$.

7. Let $R$ be a ring which is generated (as a (left) $R$-module) by its minimal left ideals (i.e. $R$ is *semi-simple*).\
   a. Prove that $R$ is the direct sum of a {\bf finite} number of minimal left ideals.\
   b. Prove that every simple $R$-module is isomorphic to a left ideal of $R$.

8. Let $R$ be a commutative ring.  Prove that an element of $R$ is nilpotent if and only if it belongs to every prime ideal of $R$.


<!-- 
SOLUTION TO 3.
    \begin{solution}
      This is simply the statement that a PID is Noetherian.  It is proved as follows:
      Let $J = \bigcup J_i$ and check that $J$ is an ideal of $R$.  Since $R$ is a PID,
      $J$ is principal, or ``one-generated.''  That is, $J = Ra$ for some $a\in R$. 
      Now $a\in Ra = \bigcup J_i$ implies $a \in J_n$ for some $n\in \N$.  Therefore, as
      $Ra$ is the smallest ideal containing $a$, we have $Ra \subseteq J_n \subseteq
      \bigcup J_i = Ra$, and similarly for all $J_i$ with $i\geq n$.  \qed
    \end{solution} 

SOLUTION TO 4.
    \begin{solution}
      In fact, if $M = K \oplus L$, then \emph{every} direct sum decomposition 
      $M = K \oplus J$ is of this form.  That is,\footnote{I write $1_M - \varphi$
        instead of $1_M + \varphi$ because the former seems a bit more natural to me, 
        but it makes no real difference.} $J = (1_M - \varphi)(L)$, for
      some $\varphi \in \Hom_R(L,K)$.  (The proof of this fact is easy, but it is not
      needed for this problem.)\footnote{See Kasch and Mader \cite{Kasch:2004}, page 4, 
        or better yet, work out the details over dinner.}

      Fix $m\in M$.  Then $m = k + l$ for some $k\in K$ and $l\in L$, and $\varphi(l) \in
      K$.  Therefore,
      \[ m = k + l = k - \varphi(l) + l + \varphi(l) = k' + (1_M + \varphi)(l).\]
      This shows that we can write any $m\in M$ as a sum $m = u+v$ with $u \in K$ and 
      $v\in (1_M + \varphi)(L)$.  Thus $M = K + (1_M + \varphi)(L)$. To show that the sum
      is direct, suppose $m$ belongs to $K \cap (1_M + \varphi)(L)$.  Then $m = k = 
      l + \varphi(l)$, for some $k \in K$ and $l\in L$.  Thus, $l = k-\varphi(l)\in K$,
      which puts $l \in K\cap L = \{0\}$, so $\varphi(l) = \varphi(0) = 0$, since
      $\varphi$ is a homomorphism. Therefore, $m = l + \varphi(l) = 0$, 
      and we have shown $M = K \oplus (1_M + \varphi)(L)$.
      % \footnote{We could just as easily have shown $M = K \oplus (1_M - \varphi)(L)$.}
      \qed
    \end{solution}

SOLUTION TO 5.
    \begin{solution}
      The natural maps are 
      \[      f: \frac{M\cap K}{N\cap K} \ni x \mapsto x+ N \in M/N      \]
      and
      \[      g: M/N \ni x+N \mapsto x+ (N+ K) \in \frac{M+ K}{N+ K}.      \]
      It is easy to check that these are well-defined homomorphisms. To see that $f$ is injective, consider
      \[      \ker(f) = \{x + (N\cap K)| x\in M\cap K \text{ and } x+N = \0\}
      % = \{x + (N\cap K)| x\in M\cap K \cap N\}
      = \{x + (N\cap K)| x\in N\cap K\} = \{\0\},      \]
      where the first $\0$ denotes $N$ (the zero of $M/N$), while the second $\0$ denotes ${N\cap K}$ (the zero of $\frac{M\cap K}{N\cap K}$).
      To see that $g$ is surjective, consider $\im(g) = \{x + (N+ K)| x\in M\} = M/(N+K)$, and note that $x + (N+ K) = x+y+ (N+ K)$ for any $y \in K$, so $M/(N+K)= (M+K)/(N+K)$.

      It remains to show that $\im(f) = \ker(g)$, and, as we see below, this turns out to be equivalent to 
      \\[6pt] 
      \underline{The Modular Law}\footnote{In
        lattice theory, we say that a lattice is \emph{modular} if it satisfies the \emph{modular law}: for elements $a, b, c$ of the lattice, if $a\leq b$, 
        then $b\meet (a\join c) = a \join (b \meet c)$.  Not coincidentally, the lattice of submodules of a module satisfies the modular law (where join is $+$ and meet is $\cap$).  
        Alas, mathematical terminology is not always perverse!}  If $N, M, K$ are submodules of some module, and $N\leq M$, then 
      \begin{equation}
        \label{eq:modular} M\cap (N+K) = N+ (M\cap K).
      \end{equation}
      This law is easy to prove by checking both inclusions; that is, consider an element of each side of~(\ref{eq:modular}) and show it is contained in the other side.

      Finally, observe,
       \begin{align*}
        \ker(g) &= \{x + N \in M/N| x\in N+K \}= \{x + N | x\in M \text{ and } x\in N+K \} \\
        &= \{x + N | x\in M \cap (N+K) \} = \{x + N | x\in N + (M \cap K) \} \quad \text{(the modular law)}\\
        &= \{x + N | x\in M \cap K \} = \im(f).
      \end{align*}
      \qed
    \end{solution}
    {\bf Remark:} The modular law is sometimes called the \emph{Dedekind identity}.  This identity, and its consequence, $\im(f) = \ker(g)$, is the crux of problem~\ref{item:modular}.  In fact, Kasch and Mader (\cite{Kasch:2004}, page 5) call the exact sequence 
    \[
    0 \longrightarrow \frac{M\cap K}{N\cap K}
    \longrightarrow \frac{M}{N} 
    \longrightarrow \frac{M+ K}{N+ K}
    \longrightarrow 0
    \]
    ``a useful and attractive version of the Dedekind identity.''
    

SOLUTION TO 7.
    \begin{solution}
      \begin{enumerate}[{\bf a.}]
      \item Assume the left regular $R$-module, $_RR$, is semi-simple, by which we mean here
        that 
        \begin{equation}
          \label{eq:semisimple}
          R = \bigoplus_{i\in I} A_i
        \end{equation}
        for some collection $\{A_i | i\in I\}$ of minimal left ideals of $R$.  We
        assume that all rings are unital, so $1\in R$.  Note that, although the direct
        sum~(\ref{eq:semisimple}) may be infinite, each $r \in R$ is a sum of finitely
        many elements from the set $\bigcup \{A_i | i\in I\}$.  In particular, 
        $1 = a_{i_1}+\cdots +a_{i_n}$ for some finite collection of indices 
        $\{i_1,\dots, i_n\}\subseteq I$
        and $a_{i_j} \in A_{i_j}$.  Therefore, 
        \[
        R = R 1 = R(a_{i_1}+\cdots +a_{i_n}) \subseteq \bigoplus_{j=1}^n A_{i_j} 
        \subseteq \bigoplus_{i\in I} A_i = R,
        \]
        which proves that $R$ is the finite direct sum $\bigoplus_{j=1}^n A_{i_j}$.
        \qed
      \end{enumerate}
    \end{solution}


SOLUTION TO 8.
    \begin{solution}
      If $s\in R$ is nilpotent, then $s^n = 0$ for some
      $n\in \N$.  In particular, $s^n = 0 \in P$ for any ideal $P$ of $R$.  If $P$ is
      prime, then $s^n \in P$ implies $s\in P$.

      To prove the converse, recall the following useful theorem:\footnote{This is
        proved in the appendix; see Theorem \ref{thm:primemult}.} 
      \\[6pt]
      {\it Theorem:} If $S$ is a multiplicative subset of a ring $R$ which is disjoint from an ideal $I$ of
      $R$, then there exists an ideal $P$ which is maximal in the set of all ideals $R$
      disjoint from $S$ and containing $I$.  Furthermore, any such ideal $P$ is
      prime.\\[6pt]
      If $s\in R$ is not nilpotent, consider the set $S = \{s, s^2, s^3, \dots\}$.
      Clearly this is a multiplicative set which is disjoint from the ideal $(0)$.
      The theorem then gives a prime ideal $P$ disjoint from $S$.  In particular,
      $s\notin P$.
      \qed

      (See also April '08 (2d).)
    \end{solution}

\end{enumerate}





1. Define “injective module.” Prove: The module $Q$ is injective if every diagram with exact row
$$\xymatrix{0 \ar[r] & P' \ar@{->}[d]_{\varphi} \ar[r]& P \\
      & Q & }$$ with [**projective**]{} $P$ is embeddable in a
commutative diagram
$$\xymatrix{0 \ar[r] & P' \ar@{->}[d]_{\varphi} \ar[r]& P \\
      & Q & }$$

Let $R$ be a commutative ring with identity. Recall that an ideal
$P\subset R$ is said to be *prime* if $P\neq R$ and $ab \in P$ implies
$a\in P$ or $b\in P$. Let $J\subseteq R$ be an ideal.

Show that $J$ is prime if and only if $R/J$ is an integral domain. Show
that $J$ is maximal if and only if $R/J$ is a field.

This is problem 2 of the April 2008 exam. (See section \[sec:April2008\]
below.)

Let $R$ be a principal ideal domain. Let $J_1, J_2, \dots$ be ideals in
$R$ such that
$$J_1 \subseteq J_2 \subseteq \cdots \subseteq J_i \subseteq J_{i+1}\subseteq \cdots$$
Show that there is an integer $n\geq 1$ such that $J_i = J_n$ for all
$i\geq n$.

This is simply the statement that a PID is Noetherian. It is proved as
follows: Let $J = \bigcup J_i$ and check that $J$ is an ideal of $R$.
Since $R$ is a PID, $J$ is principal, or “one-generated.” That is,
$J = Ra$ for some $a\in R$. Now $a\in Ra = \bigcup J_i$ implies
$a \in J_n$ for some $n\in \N$. Therefore, as $Ra$ is the smallest ideal
containing $a$, we have $Ra \subseteq J_n \subseteq
      \bigcup J_i = Ra$, and similarly for all $J_i$ with $i\geq n$.

Let $R$ be a ring and $M$ a (left) $R$-module. Suppose $M = K \oplus L$
and $\varphi$ is an $R$-endomorphism of $M$ with the property that
$\varphi(L)\subseteq
  K$. Prove that $M = K \oplus (1_M + \varphi)(L)$.

In fact, if $M = K \oplus L$, then *every* direct sum decomposition
$M = K \oplus J$ is of this form. That is,[^1] $J = (1_M - \varphi)(L)$,
for some $\varphi \in \Hom_R(L,K)$. (The proof of this fact is easy, but
it is not needed for this problem.)[^2]

Fix $m\in M$. Then $m = k + l$ for some $k\in K$ and $l\in L$, and
$\varphi(l) \in
      K$. Therefore,
$$m = k + l = k - \varphi(l) + l + \varphi(l) = k' + (1_M + \varphi)(l).$$
This shows that we can write any $m\in M$ as a sum $m = u+v$ with
$u \in K$ and $v\in (1_M + \varphi)(L)$. Thus
$M = K + (1_M + \varphi)(L)$. To show that the sum is direct, suppose
$m$ belongs to $K \cap (1_M + \varphi)(L)$. Then $m = k = 
      l + \varphi(l)$, for some $k \in K$ and $l\in L$. Thus,
$l = k-\varphi(l)\in K$, which puts $l \in K\cap L = \{0\}$, so
$\varphi(l) = \varphi(0) = 0$, since $\varphi$ is a homomorphism.
Therefore, $m = l + \varphi(l) = 0$, and we have shown
$M = K \oplus (1_M + \varphi)(L)$.

\[item:modular\] Let $R$ be any ring, $M, N, K$ submodules of some
$R$-module such that $N\leq M$. Prove that the sequence
$$0 \longrightarrow \frac{M\cap K}{N\cap K}
  \longrightarrow \frac{M}{N} 
  \longrightarrow \frac{M+ K}{N+ K}
  \longrightarrow 0$$ is exact where the maps are the natural (obvious)
ones.

The natural maps are
$$f: \frac{M\cap K}{N\cap K} \ni x \mapsto x+ N \in M/N$$ and
$$g: M/N \ni x+N \mapsto x+ (N+ K) \in \frac{M+ K}{N+ K}.$$ It is easy
to check that these are well-defined homomorphisms. To see that $f$ is
injective, consider
$$\ker(f) = \{x + (N\cap K)| x\in M\cap K \text{ and } x+N = \0\}
      % = \{x + (N\cap K)| x\in M\cap K \cap N\}
      = \{x + (N\cap K)| x\in N\cap K\} = \{\0\},$$ where the first $\0$
denotes $N$ (the zero of $M/N$), while the second $\0$ denotes
${N\cap K}$ (the zero of $\frac{M\cap K}{N\cap K}$). To see that $g$ is
surjective, consider $\mathrm{im}(g) = \{x + (N+ K)| x\in M\} = M/(N+K)$, and
note that $x + (N+ K) = x+y+ (N+ K)$ for any $y \in K$, so $M/(N+K)=
      (M+K)/(N+K)$.

It remains to show that $\mathrm{im}(f) = \ker(g)$, and, as we see below, this
turns out to be equivalent to\
[^3] If $N, M, K$ are submodules of some module, and $N\leq M$, then
$$\label{eq:modular}
        M\cap (N+K) = N+ (M\cap K).$$ This law is easy to prove by
checking both inclusions; that is, consider an element of each side
of (\[eq:modular\]) and show it is contained in the other side.

Finally, observe, $$\begin{aligned}
        \ker(g) &= \{x + N \in M/N| x\in N+K \}= \{x + N | x\in M \text{ and } x\in N+K \} \\
        &= \{x + N | x\in M \cap (N+K) \} = \{x + N | x\in N + (M \cap K) \} \quad
        \text{(the modular law)}\\
        &= \{x + N | x\in M \cap K \} = \mathrm{im}(f).
      \end{aligned}$$ The modular law is sometimes called the *Dedekind
identity*. This identity, and its consequence, $\mathrm{im}(f) = \ker(g)$, is
the crux of problem \[item:modular\]. In fact, Kasch and Mader
([@Kasch:2004], page 5) call the exact sequence
$$0 \longrightarrow \frac{M\cap K}{N\cap K}
    \longrightarrow \frac{M}{N} 
    \longrightarrow \frac{M+ K}{N+ K}
    \longrightarrow 0$$ “a useful and attractive version of the Dedekind
identity.”

Let $F$ be a field and let $R = F(X,Y]$ be the polynomial ring over $F$
in indeterminates $X, Y$. Let $\alpha, \beta \in F$, and let
$\varphi : R\rightarrow F$ be defined by
$\varphi(f(X,Y)) = f(\alpha, \beta)$ for all polynomials $f(X,Y)\in R$.
Show that $\ker(\varphi) = (x-\alpha, y-\beta)$.

Let $R$ be a ring which is generated (as a (left) $R$-module) by its
minimal left ideals ($R$ is *semi-simple*).

Prove that $R$ is the direct sum of a [**finite**]{} number of minimal
left ideals. Prove that every simple $R$-module is isomorphic to a left
ideal of $R$.

Assume the left regular $R$-module, $_RR$, is semi-simple, by which we
mean here that $$\label{eq:semisimple}
          R = \bigoplus_{i\in I} A_i$$ for some collection
$\{A_i | i\in I\}$ of minimal left ideals of $R$. We assume that all
rings are unital, so $1\in R$. Note that, although the direct
sum (\[eq:semisimple\]) may be infinite, each $r \in R$ is a sum of
finitely many elements from the set $\bigcup \{A_i | i\in I\}$. In
particular, $1 = a_{i_1}+\cdots +a_{i_n}$ for some finite collection of
indices $\{i_1,\dots, i_n\}\subseteq I$ and $a_{i_j} \in A_{i_j}$.
Therefore,
$$R = R 1 = R(a_{i_1}+\cdots +a_{i_n}) \subseteq \bigoplus_{j=1}^n A_{i_j} 
        \subseteq \bigoplus_{i\in I} A_i = R,$$ which proves that $R$ is
the finite direct sum $\bigoplus_{j=1}^n A_{i_j}$.

Let $R$ be a commutative ring. Prove that an element of $R$ is nilpotent
if and only if it belongs to every prime ideal of $R$.

If $s\in R$ is nilpotent, then $s^n = 0$ for some $n\in \N$. In
particular, $s^n = 0 \in P$ for any ideal $P$ of $R$. If $P$ is prime,
then $s^n \in P$ implies $s\in P$.

To prove the converse, recall the following useful theorem:[^4]\
[*Theorem:*]{} If $S$ is a multiplicative subset of a ring $R$ which is
disjoint from an ideal $I$ of $R$, then there exists an ideal $P$ which
is maximal in the set of all ideals $R$ disjoint from $S$ and containing
$I$. Furthermore, any such ideal $P$ is prime.\
If $s\in R$ is not nilpotent, consider the set
$S = \{s, s^2, s^3, \dots\}$. Clearly this is a multiplicative set which
is disjoint from the ideal $(0)$. The theorem then gives a prime ideal
$P$ disjoint from $S$. In particular, $s\notin P$.

(See also April ’08 (2d).)

[^1]: I write $1_M - \varphi$ instead of $1_M + \varphi$ because the
    former seems a bit more natural to me, but it makes no real
    difference.

[^2]: See Kasch and Mader [@Kasch:2004], page 4, or better yet, work out
    the details over dinner.

[^3]: In lattice theory, we say that a lattice is *modular* if it
    satisfies the *modular law*: for elements $a, b, c$ of the lattice,
    if $a\leq b$, then $b\meet (a\join c) = a \join (b \meet c)$. Not
    coincidentally, the lattice of submodules of a module satisfies the
    modular law (where join is $+$ and meet is $\cap$). Alas,
    mathematical terminology is not always perverse!

[^4]: This is proved in the appendix; see Theorem \[thm:primemult\].




















    -->
